theories/monoidal_def.v
@@ -6,33 +6,35 @@ Local Open Scope cat_scope.
 
 (** ** premonoidal categories (i.e., without coherence) *)
 
-#[primitive] HB.mixin Record IsPreMonoidal 𝐂 of cat 𝐂 := {
+(* we define them in several steps in order to setup notations along the way *)
+#[primitive] HB.mixin Record HasMonoidalOps 𝐂 of cat 𝐂 := {
     #[canonical=no] unit: 𝐂;
     #[canonical=no] tensor: Functor (𝐂*𝐂)%type 𝐂;
-    
-    (* w.r.t nlab: https://ncatlab.org/nlab/show/monoidal+category
-       assoc = α, unitl = λ, unitr = ρ *)
-    #[canonical=no] assoc_:
-    tensor ∘ times tensor idmap
-      ≈
-    tensor ∘ times idmap tensor ∘ (prod_assoc _ _ _)¹;
-    #[canonical=no] unitl_: 
-    tensor ∘ (times (functor_cst unit) idmap)
-      ≈
-    (@prod_unitl Cat _)¹;
-    #[canonical=no] unitr_: 
-    tensor ∘ (times idmap (functor_cst unit))
-      ≈
-    (@prod_unitr Cat _)¹;
   }.
-#[short(type="PreMonoidalCat")]
-HB.structure Definition premonoidalcat := { 𝐂 of uip 𝐂 & cat 𝐂 & IsPreMonoidal 𝐂 }.
+#[short(type="MonoidalOpsCat")]
+HB.structure Definition monoidalopscat := { 𝐂 of cat 𝐂 & HasMonoidalOps 𝐂 }.
 
-Definition tensor11 {𝐂: PreMonoidalCat} (A B: 𝐂): 𝐂 := app11 tensor A B.
+Definition tensor11 {𝐂: MonoidalOpsCat} (A B: 𝐂): 𝐂 := app11 tensor A B.
 Infix "⊗" := tensor11: cat_scope.
-Definition tensor22 {𝐂: PreMonoidalCat} {A B C D: 𝐂} (f: A~>B) (g: C~>D): A⊗C ~> B⊗D := app22 tensor f g.
+Definition tensor22 {𝐂: MonoidalOpsCat} {A B C D: 𝐂} (f: A~>B) (g: C~>D): A⊗C ~> B⊗D := app22 tensor f g.
 Infix "·" := tensor22: cat_scope.
 
+#[primitive] HB.mixin Record IsPreMonoidal 𝐂 of monoidalopscat 𝐂 := {
+    (* w.r.t nlab: https://ncatlab.org/nlab/show/monoidal+category
+       assoc = α, unitl = λ, unitr = ρ *)
+    #[canonical=no] assoc_: forall A B C: 𝐂, (A⊗B)⊗C ≃ A⊗(B⊗C);
+    #[canonical=no] unitl_: forall A: 𝐂, unit⊗A ≃ A;
+    #[canonical=no] unitr_: forall A: 𝐂, A⊗unit ≃ A;
+
+    #[canonical=no] ntx_assoc_: forall (A B C A' B' C': 𝐂) f g h,
+      assoc_ A' B' C' ∘ (f · g) · h ≡ f · (g · h) ∘ assoc_ A B C;
+    #[canonical=no] ntx_unitl_: forall (A A': 𝐂) f,
+      unitl_ A' ∘ unit · f ≡ f ∘ unitl_ A ;
+    #[canonical=no] ntx_unitr_: forall (A A': 𝐂) f,
+      unitr_ A' ∘ f · unit ≡ f ∘ unitr_ A ;
+  }.
+#[short(type="PreMonoidalCat")]
+HB.structure Definition premonoidalcat := { 𝐂 of uip 𝐂 & monoidalopscat 𝐂 & IsPreMonoidal 𝐂 }.
 
 (** extension of the normalisation tactic from cat.v *)
 
@@ -49,26 +51,6 @@ Section s.
   
 Context {𝐂: PreMonoidalCat}.
 Implicit Types A B C D: 𝐂.
-
-Definition assoc A B C: (A ⊗ B) ⊗ C ~> A ⊗ (B ⊗ C) := assoc_ (A,B,C).
-Definition unitl A: unit ⊗ A ~> A := unitl_ (tt,A). 
-Definition unitr A: A ⊗ unit ~> A := unitr_ (A,tt).
-Arguments assoc: simpl never.
-Arguments unitl: simpl never.
-Arguments unitr: simpl never.
-HB.instance Definition _ A B C := iso.on (assoc A B C). 
-HB.instance Definition _ A := iso.on (unitl A). 
-HB.instance Definition _ A := iso.on (unitr A). 
-
-Definition assoc' A B C: A ⊗ (B ⊗ C) ~> (A ⊗ B) ⊗ C := (assoc A B C)⁻¹.
-Definition unitl' A: A ~> unit ⊗ A := (unitl A)⁻¹.
-Definition unitr' A: A ~> A ⊗ unit := (unitr A)⁻¹.
-Arguments assoc': simpl never.
-Arguments unitl': simpl never.
-Arguments unitr': simpl never.
-HB.instance Definition _ A B C := iso.on (assoc' A B C). 
-HB.instance Definition _ A := iso.on (unitl' A). 
-HB.instance Definition _ A := iso.on (unitr' A). 
 
 Lemma tensor_id {A B}: idmap A · idmap B ≡ idmap (A⊗B). 
 Proof. exact: (@Fidmap _ _ _ (A,B)). Qed.
@@ -110,31 +92,56 @@ Definition _iso_tens {A A' B B'} (i: A ≃ A') (j: B ≃ B'): IsIso _ (A⊗B) (A
   @_functor_iso _ _ tensor (A,B) (A',B') (pair_iso i j). 
 HB.instance Definition _ {A A' B B'} (i: A ≃ A') (j: B ≃ B') := _iso_tens i j. 
 
+
+Definition assoc A B C: (A ⊗ B) ⊗ C ~> A ⊗ (B ⊗ C) := (assoc_ A B C)¹.
+Definition unitl A: unit ⊗ A ~> A := (unitl_ A)¹.
+Definition unitr A: A ⊗ unit ~> A := (unitr_ A)¹.
+Arguments assoc: simpl never.
+Arguments unitl: simpl never.
+Arguments unitr: simpl never.
+HB.instance Definition _ A B C := iso.on (assoc A B C). 
+HB.instance Definition _ A := iso.on (unitl A). 
+HB.instance Definition _ A := iso.on (unitr A). 
+
+Definition assoc' A B C: A ⊗ (B ⊗ C) ~> (A ⊗ B) ⊗ C := (assoc A B C)⁻¹.
+Definition unitl' A: A ~> unit ⊗ A := (unitl A)⁻¹.
+Definition unitr' A: A ~> A ⊗ unit := (unitr A)⁻¹.
+Arguments assoc': simpl never.
+Arguments unitl': simpl never.
+Arguments unitr': simpl never.
+HB.instance Definition _ A B C := iso.on (assoc' A B C). 
+HB.instance Definition _ A := iso.on (unitl' A). 
+HB.instance Definition _ A := iso.on (unitr' A). 
+
+
 Lemma ntx_assoc [A B A' B' A'' B''] (f: A ~> B) (g: A' ~> B') (h: A'' ~> B''):
   assoc _ _ _ ∘ (f · g) · h ≡ f · (g · h) ∘ assoc _ _ _.
-Proof. exact: (@natural _ _ _ _ (assoc_¹) (_,_,_) (_,_,_) (f,g,h)). Qed.
+Proof. exact: ntx_assoc_. Qed.
 
 Lemma ntx_assoc' [A B A' B' A'' B''] (f: A ~> B) (g: A' ~> B') (h: A'' ~> B''):
   assoc' _ _ _ ∘ f · (g · h) ≡ (f · g) · h ∘ assoc' _ _ _.
-Proof. exact: (@natural _ _ _ _ (assoc_⁻¹) (_,_,_) (_,_,_) (f,g,h)). Qed.
+Proof. by rewrite iso_tgt_l compoA -iso_src_l ntx_assoc. Qed.
 
 Lemma ntx_unitl [A B] (f: A ~> B): unitl _ ∘ unit · f ≡ f ∘ unitl _.
-Proof. exact: (@natural _ _ _ _ (unitl_¹) (tt,A) (tt,B) (idmap,f)). Qed.
+Proof. exact: ntx_unitl_. Qed.
 
 Lemma ntx_unitl' [A B] (f: A ~> B): unitl' _ ∘ f ≡ unit · f ∘ unitl' _.
-Proof. exact: (@natural _ _ _ _ (unitl_⁻¹) (tt,A) (tt,B) (idmap,f)). Qed.
+Proof. by rewrite iso_tgt_l compoA -iso_src_l ntx_unitl. Qed.
 
 Lemma ntx_unitr [A B] (f: A ~> B): unitr _ ∘ f · unit ≡ f ∘ unitr _.
-Proof. exact: (@natural _ _ _ _ (unitr_¹) (A,tt) (B,tt) (f,idmap)). Qed.
+Proof. exact: ntx_unitr_. Qed.
 
 Lemma ntx_unitr' [A B] (f: A ~> B): unitr' _ ∘ f ≡ f · unit ∘ unitr' _.
-Proof. exact: (@natural _ _ _ _ (unitr_⁻¹) (A,tt) (B,tt) (f,idmap)). Qed.
+Proof. by rewrite iso_tgt_l compoA -iso_src_l ntx_unitr. Qed.
 
 
 
 Definition tensor11_eq A A' B B' (a: A=A') (b: B=B'): A⊗B = A'⊗B'.
   by rewrite a b.
 Defined.
+Lemma tensor11_eq_sym A A' B B' (a: A=A') (b: B=B'):
+  tensor11_eq (esym a) (esym b) = esym (tensor11_eq a b).
+Proof. by destruct a, b. Qed.
 Lemma hcast_tensor A A' B B' C C' D D' (f: A ~> B) (g: C ~> D)
   (a: A=A') (b: B=B') (c: C=C') (d: D=D'):
   hcast' f a b · hcast' g c d = hcast' (f · g) (tensor11_eq a c) (tensor11_eq b d).
@@ -149,8 +156,8 @@ Proof. by destruct a; destruct b; destruct c. Qed.
 Lemma hcast_assoc_ A A' B B' C C' p q (a: A=A') (b: B=B') (c: C=C'):
   hcast' (assoc A B C) p q = assoc A' B' C'.
 Proof.
-  rewrite (UIP_ob _ _ p (tensor11_eq (tensor11_eq a b) c)).
-  rewrite (UIP_ob _ _ q (tensor11_eq a (tensor11_eq b c))).
+  rewrite (UIP_ob p (tensor11_eq (tensor11_eq a b) c)).
+  rewrite (UIP_ob q (tensor11_eq a (tensor11_eq b c))).
   exact/hcast_assoc.
 Qed.
 Lemma hcast_assoc' A A' B B' C C' (a: A=A') (b: B=B') (c: C=C'):
@@ -162,8 +169,8 @@ Proof. by destruct a; destruct b; destruct c. Qed.
 Lemma hcast_assoc'_ A A' B B' C C' p q (a: A=A') (b: B=B') (c: C=C'):
   hcast' (assoc' A B C) p q = assoc' A' B' C'.
 Proof.
-  rewrite (UIP_ob _ _ p (tensor11_eq a (tensor11_eq b c))).
-  rewrite (UIP_ob _ _ q (tensor11_eq (tensor11_eq a b) c)).
+  rewrite (UIP_ob p (tensor11_eq a (tensor11_eq b c))).
+  rewrite (UIP_ob q (tensor11_eq (tensor11_eq a b) c)).
   exact/hcast_assoc'.
 Qed.
 Lemma hcast_unitl A A' (a: A=A'):
@@ -172,7 +179,7 @@ Proof. by destruct a. Qed.
 Lemma hcast_unitl_ A A' (a: A=A') p:
   hcast' (unitl A) p a = unitl A'.
 Proof.
-  rewrite (UIP_ob _ _ p (tensor11_eq eq_refl a)).
+  rewrite (UIP_ob p (tensor11_eq eq_refl a)).
   exact/hcast_unitl.
 Qed.
 Lemma hcast_unitl' A A' (a: A=A'):
@@ -181,7 +188,7 @@ Proof. by destruct a. Qed.
 Lemma hcast_unitl'_ A A' (a: A=A') p:
   hcast' (unitl' A) a p = unitl' A'.
 Proof.
-  rewrite (UIP_ob _ _ p (tensor11_eq eq_refl a)).
+  rewrite (UIP_ob p (tensor11_eq eq_refl a)).
   exact/hcast_unitl'.
 Qed.
 Lemma hcast_unitr A A' (a: A=A'):
@@ -190,7 +197,7 @@ Proof. by destruct a. Qed.
 Lemma hcast_unitr_ A A' (a: A=A') p:
   hcast' (unitr A) p a = unitr A'.
 Proof.
-  rewrite (UIP_ob _ _ p (tensor11_eq a eq_refl)).
+  rewrite (UIP_ob p (tensor11_eq a eq_refl)).
   exact/hcast_unitr.
 Qed.
 Lemma hcast_unitr' A A' (a: A=A'):
@@ -199,11 +206,11 @@ Proof. by destruct a. Qed.
 Lemma hcast_unitr'_ A A' (a: A=A') p:
   hcast' (unitr' A) a p = unitr' A'.
 Proof.
-  rewrite (UIP_ob _ _ p (tensor11_eq a eq_refl)).
+  rewrite (UIP_ob p (tensor11_eq a eq_refl)).
   exact/hcast_unitr'.
 Qed.
 
-(** * class for automatic inferrence of McLane isomorphisms  *)
+(** * class for automatic inferrence of MacLane isomorphisms  *)
 
 Class Bridge A B := mcl: A ≃ B.
 Notation mcl_ b := (@mcl _ _ b) (only parsing).
@@ -229,8 +236,18 @@ Definition blocked_unitl' {A}: _ ≃ _ := unitl' A.
 Definition blocked_unitr {A}: _ ≃ _ := unitr A.
 Definition blocked_unitr' {A}: _ ≃ _ := unitr' A.
 
-(** temporay resolution, to be overriden in [monoidal_gmclane]  *)
+(** temporay resolution, to be overriden in [monoidal_gmaclane]  *)
 Local Hint Extern 0 (auto_eqv _ _) => unfold auto_eqv; simpl; cat: typeclass_instances.
+
+Lemma bexchange {A B B_ C A' B' B_' C'}
+  (i: A ~> B) (j: B_ ~> C)
+  (i': A' ~> B') (j': B_' ~> C') (m n n': _ ≃ _)
+  (H: iso.sort m ≡ n·n'):
+  bcomp (i·i') (j·j') m ≡ (bcomp i j n) · (bcomp i' j' n').
+Proof.
+  rewrite /bcomp-!lock H.
+  by rewrite 2!exchange. 
+Qed.
 
 Lemma tensor_bcomp {A B C D A' B' C' D'}
   (i: A ~> B) m (j: C ~> D)
