theories/monoidal_gmaclane.v
@@ -1,22 +1,25 @@
-(** * inferrence of (generalised) McLane isomorphisms *)
+(** * inferrence of (generalised) MacLane isomorphisms,
+      generalised MacLane's coherence theorem, and associated tactic *)
 
-Require Import arity monoidal_def monoidal_mclane.
+Require Import arity monoidal_def monoidal_maclane.
 From elpi Require Import elpi coercion.
 
 Local Open Scope cat_scope. 
 
 Section s.
 Context {X: Type}.
+
+(** generalised tensor-tree expressions *)
 Inductive gtree :=
 | gt_ob(x: X)
-| gt_tree (t: tree X)           (* remove? *)
+| gt_tree(t: tree X)           (* remove? *)
 | gt_unit
-| gt_tens(s t: gtree)
+| gt_tensor(s t: gtree)
 | gt_trees(h: gtrees)
 with gtrees :=
-| gt_ar (a: arity X)
-| gt_nf (t: tree X)
-| gt_gnf (t: gtree)
+| gt_ar(a: arity X)
+| gt_nf(t: tree X)
+| gt_gnf(t: gtree)
 | gt_nil
 | gt_cons(s: gtree)(h: gtrees)
 | gt_app (h k: gtrees).
@@ -26,7 +29,7 @@ Fixpoint gNorm t: norm X :=
   | gt_ob x => cons x
   | gt_tree t => Norm t
   | gt_unit => n_id
-  | gt_tens s t => n_tensor (gNorm s) (gNorm t)
+  | gt_tensor s t => n_tensor (gNorm s) (gNorm t)
   | gt_trees l => gNorm' l
   end
 with gNorm' t: norm X :=
@@ -51,13 +54,13 @@ Proof.
   destruct t=>//=. exact/esym/aappA. exact/Norm_app. by rewrite gNorm'_app. by rewrite gNorm'_app. 
 Defined.
 
-Lemma gNf_tensor a b: gNf (gt_tens a b) = gNf a ++ gNf b.
+Lemma gNf_tensor a b: gNf (gt_tensor a b) = gNf a ++ gNf b.
 Proof. by rewrite /gNf -gNorm_app. Defined.
 
 Fixpoint tensor_arity (l: arity X) (k: tree X): tree X :=
   match l with
   | nil => k
-  | cons x q => t_tens (t_ob x) (tensor_arity q k)
+  | cons x q => t_tensor (t_ob x) (tensor_arity q k)
   end.
 
 Lemma tensor_arity_app h k t: tensor_arity (h++k) t = tensor_arity h (tensor_arity k t).
@@ -70,7 +73,7 @@ Fixpoint tree_gtree t :=
   match t with
   | t_ob x => gt_ob x
   | t_unit => gt_unit
-  | t_tens s t => gt_tens (tree_gtree s) (tree_gtree t)
+  | t_tensor s t => gt_tensor (tree_gtree s) (tree_gtree t)
   end.
 
 End s.
@@ -88,7 +91,7 @@ Fixpoint eval_gtree a: 𝐂 :=
   | gt_ob x => x
   | gt_tree t => t
   | gt_unit => unit
-  | gt_tens a b => eval_gtree a ⊗ eval_gtree b
+  | gt_tensor a b => eval_gtree a ⊗ eval_gtree b
   | gt_trees t => eval_arity (eval_gtrees t)
   end
 with eval_gtrees t: arity 𝐂 :=
@@ -106,7 +109,7 @@ Fixpoint gtree_tree (t: gtree 𝐂): tree 𝐂 :=
   | gt_ob x => t_ob x
   | gt_tree t => t
   | gt_unit => t_unit
-  | gt_tens s t => t_tens (gtree_tree s) (gtree_tree t)
+  | gt_tensor s t => t_tensor (gtree_tree s) (gtree_tree t)
   | gt_trees h => gtrees_tree h t_unit
   end
 with gtrees_tree (t: gtrees 𝐂) k: tree 𝐂 :=
@@ -115,7 +118,7 @@ with gtrees_tree (t: gtrees 𝐂) k: tree 𝐂 :=
   | gt_nf t => tensor_arity (Nf t) k
   | gt_gnf t => tensor_arity (gNf t) k
   | gt_nil => k
-  | gt_cons s t => t_tens (gtree_tree s) (gtrees_tree t k)
+  | gt_cons s t => t_tensor (gtree_tree s) (gtrees_tree t k)
   | gt_app s t => gtrees_tree s (gtrees_tree t k)
   end.
 
@@ -167,87 +170,92 @@ Qed.
 Corollary gNfE t: gNf t = Nf (gtree_tree t).
 Proof. exact/gNormE. Qed.
 
-Definition gmclane a b := mclane (gtree_tree a) (gtree_tree b).
+Definition gmaclane a b := maclane (gtree_tree a) (gtree_tree b).
 
-Theorem find_gMcLane a b (e: gNf a = gNf b): gmclane a b.
+Theorem find_gMacLane a b (e: gNf a = gNf b): gmaclane a b.
 Proof.
   have{}e : Nf (gtree_tree a) = Nf (gtree_tree b) by rewrite -2!gNfE.
-  exact: find_McLane e. 
+  exact: find_MacLane e. 
 Qed.
 
-Definition iso_gmclane a b (h: gmclane a b): eval_gtree a ≃ eval_gtree b :=
-  locked (icast' (iso_mclane h) (esym (eval_gtree_tree a)) (esym (eval_gtree_tree b))).
-Definition eval_gmclane a b (h: gmclane a b): eval_gtree a ~> eval_gtree b := iso_gmclane h.
+Definition iso_gmaclane a b (h: gmaclane a b): eval_gtree a ≃ eval_gtree b :=
+  locked (icast' (iso_maclane h) (esym (eval_gtree_tree a)) (esym (eval_gtree_tree b))).
+Definition eval_gmaclane a b (h: gmaclane a b): eval_gtree a ~> eval_gtree b := iso_gmaclane h.
 
-Lemma eval_gmclaneE a b (h: gmclane a b):
-  iso.sort (iso_gmclane h) = hcast' (eval_mclane h) (esym (eval_gtree_tree a)) (esym (eval_gtree_tree b)).
-Proof. by rewrite /iso_gmclane-lock -hcast_iso. Qed.
+Lemma eval_gmaclaneE a b (h: gmaclane a b):
+  iso.sort (iso_gmaclane h) = hcast' (eval_maclane h) (esym (eval_gtree_tree a)) (esym (eval_gtree_tree b)).
+Proof. by rewrite /iso_gmaclane-lock -hcast_iso. Qed.
 
-Coercion iso_gmclane: gmclane >-> iso.type.
+Coercion iso_gmaclane: gmaclane >-> iso.type.
 Local Coercion gtree_tree: gtree >-> tree.
 
-Definition gmcl_id a: gmclane a a := mcl_id a. 
-Definition gmcl_comp a b c (f: gmclane a b) (g: gmclane b c): gmclane a c := mcl_comp f g. 
-Definition gmcl_inv a b (f: gmclane a b): gmclane b a := mcl_inv f. 
-Definition gmcl_tensor a b c d (f: gmclane a b) (g: gmclane c d): gmclane (gt_tens a c) (gt_tens b d) := mcl_tensor f g. 
-Definition gmcl_assoc a b c: gmclane (gt_tens (gt_tens a b) c) (gt_tens a (gt_tens b c)) := mcl_assoc a b c. 
+Definition gmcl_id a: gmaclane a a := mcl_id a. 
+Definition gmcl_comp a b c (f: gmaclane a b) (g: gmaclane b c): gmaclane a c := mcl_comp f g. 
+Definition gmcl_inv a b (f: gmaclane a b): gmaclane b a := mcl_inv f. 
+Definition gmcl_tensor a b c d (f: gmaclane a b) (g: gmaclane c d): gmaclane (gt_tensor a c) (gt_tensor b d) := mcl_tensor f g. 
+Definition gmcl_assoc a b c: gmaclane (gt_tensor (gt_tensor a b) c) (gt_tensor a (gt_tensor b c)) := mcl_assoc a b c. 
 Definition gmcl_assoc' a b c := gmcl_inv (gmcl_assoc a b c). 
-Definition gmcl_unitl a: gmclane (gt_tens gt_unit a) a := mcl_unitl a. 
+Definition gmcl_unitl a: gmaclane (gt_tensor gt_unit a) a := mcl_unitl a. 
 Definition gmcl_unitl' a := gmcl_inv (gmcl_unitl a). 
-Definition gmcl_unitr a: gmclane (gt_tens a gt_unit) a := mcl_unitr a. 
+Definition gmcl_unitr a: gmaclane (gt_tensor a gt_unit) a := mcl_unitr a. 
 Definition gmcl_unitr' a := gmcl_inv (gmcl_unitr a). 
 
-Definition gmcl_eq a b (e: gtree_tree a = gtree_tree b): gmclane a b :=
-  cast2' (T:=@mclane _) (mcl_id (gtree_tree a)) erefl e. 
-Definition gmcl_comp' a b b' c (f: gmclane a b) (e: gtree_tree b = gtree_tree b') (g: gmclane b' c): gmclane a c :=
+Definition gmcl_eq a b (e: gtree_tree a = gtree_tree b): gmaclane a b :=
+  cast2' (T:=@maclane _) (mcl_id (gtree_tree a)) erefl e. 
+Definition gmcl_comp' a b b' c (f: gmaclane a b) (e: gtree_tree b = gtree_tree b') (g: gmaclane b' c): gmaclane a c :=
   (gmcl_comp f (gmcl_comp (gmcl_eq e) g)).
 
-Definition gmcl_mclane s t (f: mclane s t): gmclane (tree_gtree s) (tree_gtree t) :=
+Definition gmcl_maclane s t (f: maclane s t): gmaclane (tree_gtree s) (tree_gtree t) :=
   cast2' f (esym (gtree_tree_gtree s)) (esym (gtree_tree_gtree t)).
 
-Lemma eval_gmclane_id a: gmcl_id a ≡ idmap.
-Proof. by rewrite eval_gmclaneE hcast_id. Qed.
-Lemma eval_gmclane_comp a b c (f: gmclane a b) (g: gmclane b c): gmcl_comp f g ≡ f \; g.
-Proof. by rewrite !eval_gmclaneE hcast_comp. Qed.
-Lemma eval_gmclane_inv a b (f: gmclane a b): gmcl_inv f ≡ f⁻¹.
+Lemma eval_gmaclane_id a: gmcl_id a ≡ idmap.
+Proof. by rewrite eval_gmaclaneE hcast_id. Qed.
+Lemma eval_gmaclane_comp a b c (f: gmaclane a b) (g: gmaclane b c): gmcl_comp f g ≡ f \; g.
+Proof. by rewrite !eval_gmaclaneE hcast_comp. Qed.
+Lemma eval_gmaclane_inv a b (f: gmaclane a b): gmcl_inv f ≡ f⁻¹.
 Proof.
-  rewrite eval_gmclaneE -eval_mclane_invE/=.
+  rewrite eval_gmaclaneE -eval_maclane_invE/=.
   rewrite hcast_inv. apply: inv_inj=>/=.
-  rewrite -hcast_iso. cbn. by rewrite eval_gmclaneE. 
+  rewrite -hcast_iso. cbn. by rewrite eval_gmaclaneE. 
 Qed.
-Lemma eval_gmclane_tensor a b c d (f: gmclane a b) (g: gmclane c d): gmcl_tensor f g ≡ f · g.
-Proof. rewrite !eval_gmclaneE hcast_tensor/=. exact/hcast_eqv'. Qed.
-Lemma eval_gmclane_assoc a b c: gmcl_assoc a b c ≡ assoc (eval_gtree a) (eval_gtree b) (eval_gtree c).
-Proof. rewrite !eval_gmclaneE/=hcast_assoc_//; symmetry; exact: eval_gtree_tree. Qed.
-Lemma eval_gmclane_assoc' a b c: gmcl_assoc' a b c ≡ assoc' (eval_gtree a) (eval_gtree b) (eval_gtree c).
-Proof. rewrite eval_gmclane_inv. apply: inv_inj. exact/eval_gmclane_assoc. Qed.
-Lemma eval_gmclane_unitl a: gmcl_unitl a ≡ unitl (eval_gtree a).
-Proof. rewrite !eval_gmclaneE/=hcast_unitl_//. Qed.
-Lemma eval_gmclane_unitl' a: gmcl_unitl' a ≡ unitl' (eval_gtree a).
-Proof. rewrite eval_gmclane_inv. apply: inv_inj. exact/eval_gmclane_unitl. Qed.
-Lemma eval_gmclane_unitr a: gmcl_unitr a ≡ unitr (eval_gtree a).
-Proof. rewrite !eval_gmclaneE/=hcast_unitr_//. Qed.
-Lemma eval_gmclane_unitr' a: gmcl_unitr' a ≡ unitr' (eval_gtree a).
-Proof. rewrite eval_gmclane_inv. apply: inv_inj. exact/eval_gmclane_unitr. Qed.
 
-Lemma eval_gmclane_cast a a' b b' (f: gmclane a b) aa bb:
-  iso_gmclane (@cast2' _ _ a b a' b' f aa bb) =
+Lemma eval_gmaclane_tensor a b c d (f: gmaclane a b) (g: gmaclane c d): gmcl_tensor f g ≡ f · g.
+Proof. by rewrite !eval_gmaclaneE hcast_tensor/= 2!tensor11_eq_sym. Qed.
+Lemma eval_gmaclane_assoc a b c: gmcl_assoc a b c ≡ assoc (eval_gtree a) (eval_gtree b) (eval_gtree c).
+Proof. by rewrite !eval_gmaclaneE/= -!tensor11_eq_sym hcast_assoc. Qed.
+Lemma eval_gmaclane_assoc' a b c: gmcl_assoc' a b c ≡ assoc' (eval_gtree a) (eval_gtree b) (eval_gtree c).
+Proof. rewrite eval_gmaclane_inv. apply: inv_inj. exact/eval_gmaclane_assoc. Qed.
+Lemma eval_gmaclane_unitl a: gmcl_unitl a ≡ unitl (eval_gtree a).
+Proof. rewrite !eval_gmaclaneE/=. by destruct (eval_gtree_tree a). Qed.
+Lemma eval_gmaclane_unitl' a: gmcl_unitl' a ≡ unitl' (eval_gtree a).
+Proof. rewrite eval_gmaclane_inv. apply: inv_inj. exact/eval_gmaclane_unitl. Qed.
+Lemma eval_gmaclane_unitr a: gmcl_unitr a ≡ unitr (eval_gtree a).
+Proof. rewrite !eval_gmaclaneE/=. by destruct (eval_gtree_tree a). Qed.
+Lemma eval_gmaclane_unitr' a: gmcl_unitr' a ≡ unitr' (eval_gtree a).
+Proof. rewrite eval_gmaclane_inv. apply: inv_inj. exact/eval_gmaclane_unitr. Qed.
+
+Lemma eval_gmaclane_cast a a' b b' (f: gmaclane a b) aa bb:
+  iso_gmaclane (@cast2' _ _ a b a' b' f aa bb) =
     icast' f (f_equal eval_gtree aa) (f_equal eval_gtree bb). 
 Proof. by destruct aa; destruct bb. Qed.
 
+
+
 Definition mcl_eq a b (e: gtree_tree a = gtree_tree b): eval_gtree a ~> eval_gtree b :=
   hcast' idmap (esym (eval_gtree_tree _)) (etrans (f_equal eval_tree e) (esym (eval_gtree_tree _))).
-Lemma eval_gmclane_eq a b e:
+Lemma eval_gmaclane_eq a b e:
   @gmcl_eq a b e ≡ mcl_eq e.
-Proof. rewrite /gmcl_eq !eval_gmclaneE. rewrite eval_mclane_cast hcastI/=/mcl_eq. McLane. Qed. 
+Proof. rewrite /gmcl_eq !eval_gmaclaneE. by rewrite eval_maclane_cast hcastI/=/mcl_eq etrans_id. Qed.
 
-Lemma eval_gmclane_comp' a b b' c (f: gmclane a b) e (g: gmclane b' c): gmcl_comp' f e g ≡ f \; mcl_eq e \; g.
-Proof. by rewrite 2!eval_gmclane_comp eval_gmclane_eq. Qed.
+Lemma eval_gmaclane_comp' a b b' c (f: gmaclane a b) e (g: gmaclane b' c): gmcl_comp' f e g ≡ f \; mcl_eq e \; g.
+Proof. by rewrite 2!eval_gmaclane_comp eval_gmaclane_eq. Qed.
 
-Lemma eval_gmclane_mclane s t (f: mclane s t): gmcl_mclane f ≡ hcast' (eval_mclane f) (eval_tree_gtree s) (eval_tree_gtree t).
-Proof. rewrite !eval_gmclaneE eval_mclane_cast hcastI. McLane. Qed.
+Lemma eval_gmaclane_maclane s t (f: maclane s t): gmcl_maclane f ≡ hcast' (eval_maclane f) (eval_tree_gtree s) (eval_tree_gtree t).
+Proof. rewrite !eval_gmaclaneE eval_maclane_cast hcastI. MacLane. Qed.
 
 End s.
+
+(** reification of generalised tensor tree expressions *)
 
 Ltac reify_ob A :=
   lazymatch A with
@@ -255,7 +263,7 @@ Ltac reify_ob A :=
   | ?A ⊗ ?B =>
       let a := reify_ob A in
       let b := reify_ob B in
-      constr:(gt_tens a b)
+      constr:(gt_tensor a b)
   | eval_tree ?t => constr:(gt_tree t) (* tree_gtree ? *)
   | eval_gtree ?t => constr:(t)
   | eval_arity ?L =>
@@ -281,23 +289,24 @@ with reify_ar L :=
   | ?L => constr:(gt_ar L)
   end.
 
-Ltac find_gmclane' :=
+(** final tactic for inferring MacLane isomorphisms *)
+Ltac find_gmaclane' :=
   unfold Bridge;
   match goal with
   | |- ?A ≃ ?B => 
       let a := reify_ob A in
       let b := reify_ob B in
-      refine (iso_gmclane (@find_gMcLane _ a b _))
+      refine (iso_gmaclane (@find_gMacLane _ a b _))
   | |- ?A ~> ?B => 
       let a := reify_ob A in
       let b := reify_ob B in
-      refine (eval_gmclane (@find_gMcLane _ a b _))
+      refine (eval_gmaclane (@find_gMacLane _ a b _))
   end.
 
-Ltac find_gmclane := by find_gmclane'.
-#[export] Hint Extern 0 (Bridge _ _) => find_gmclane: typeclass_instances.
+Ltac find_gmaclane := by find_gmaclane'.
+#[export] Hint Extern 0 (Bridge _ _) => find_gmaclane: typeclass_instances.
 
-Section test_find_gmclane.
+Section test_find_gmaclane.
 Context {𝐂: PreMonoidalCat}.
 Variables A B C: 𝐂.
 Variables a b c: tree 𝐂.
@@ -309,9 +318,9 @@ Check mcl: h++A⊗unit⊗B::k ~> h⊗A⊗B⊗k.
 Check (mcl: Γ++Δ ~> Γ⊗Δ) ≡ acast (mcl: Γ++Δ ~> Γ⊗unit⊗Δ).
 Check mcl: unit ⊗ Nf b ⊗ C ~> b ⊗ C.
 Check mcl: unit ⊗ gNf g ⊗ C ~> eval_gtree g ⊗ C.
-Check mcl: unit ⊗ gNf (gt_tens g g) ⊗ C ~> eval_gtree g ⊗ eval_gtree g ⊗ C. 
-Check mcl: unit ⊗ Nf (t_tens b c) ⊗ C ~> b ⊗ c ⊗ C.
-Check mcl: unit ⊗ Nf (t_tens b c) ⊗ C ~> b ⊗ Nf c ⊗ C.
+Check mcl: unit ⊗ gNf (gt_tensor g g) ⊗ C ~> eval_gtree g ⊗ eval_gtree g ⊗ C. 
+Check mcl: unit ⊗ Nf (t_tensor b c) ⊗ C ~> b ⊗ c ⊗ C.
+Check mcl: unit ⊗ Nf (t_tensor b c) ⊗ C ~> b ⊗ Nf c ⊗ C.
 Check mcl: unit ⊗ (h++k) ⊗ B ⊗ C ~> h ⊗ unit ⊗ k ⊗ B ⊗ unit ⊗ C.
 Check mcl: A ⊗ (h++B::k) ⊗ C ~> A⊗ h ⊗ B ⊗ k ⊗ unit ⊗ C.
 Check mcl: A ⊗ (h++(B⊗C)::k) ⊗ C ~> A⊗ h ⊗ B ⊗ C ⊗ k ⊗ unit ⊗ C.
@@ -322,22 +331,23 @@ Check fun (f: A ~> (B⊗unit)) (g: unit⊗B ~> A) => acast g ∘ f.
 Check fun (f: A ~> (B⊗unit)) (g: unit⊗B ~> A) => idmap ∘ g ∘∘ f.
 Check fun (f: A ~> (B⊗unit)) (g: unit⊗B ~> A) => g ∘ acast f.
 Check fun (f: A ~> (B⊗unit)) (g: B ~> A) => g ∘ mcl ∘ f.
-End test_find_gmclane.
+End test_find_gmaclane.
 
-Theorem gMcLane {𝐂: MonoidalCat} {a b: gtree 𝐂} (f g: gmclane a b): f ≡ g.
-Proof. rewrite !eval_gmclaneE. apply: hcast_eqv. exact/McLane. Qed.
+(** generalised coherence theorem  *)
+Theorem gMacLane {𝐂: MonoidalCat} {a b: gtree 𝐂} (f g: gmaclane a b): f ≡ g.
+Proof. rewrite !eval_gmaclaneE. apply: hcast_eqv. exact/MacLane. Qed.
 
-(** McLane (iso)morphisms *)
+(** MacLane (iso)morphisms *)
 
-HB.mixin Record isMcLane (𝐂: PreMonoidalCat) (A B: 𝐂) (f: A ~> B) := {
+HB.mixin Record isMacLane (𝐂: PreMonoidalCat) (A B: 𝐂) (f: A ~> B) := {
     #[canonical=no] src_gtree: gtree 𝐂; 
     #[canonical=no] tgt_gtree: gtree 𝐂; 
     #[canonical=no] srcE: eval_gtree src_gtree = A; 
     #[canonical=no] tgtE: eval_gtree tgt_gtree = B; 
-    #[canonical=no] rmcl: gmclane src_gtree tgt_gtree; 
-    #[canonical=no] rmorE: f ≡ hcast' (iso_gmclane rmcl) srcE tgtE;
+    #[canonical=no] rmcl: gmaclane src_gtree tgt_gtree; 
+    #[canonical=no] rmorE: f ≡ hcast' (iso_gmaclane rmcl) srcE tgtE;
   }.
-HB.builders Context 𝐂 a b f of isMcLane 𝐂 a b f.
+HB.builders Context 𝐂 a b f of isMacLane 𝐂 a b f.
   Definition f': b ~> a := hcast' (rmcl⁻¹) tgtE srcE.
   Program Definition _iso := @IsIso.Build 𝐂 _ _ f f' _ _.
   Next Obligation. by rewrite rmorE/f' hcast_comp isoK hcast_id. Qed.
@@ -345,31 +355,31 @@ HB.builders Context 𝐂 a b f of isMcLane 𝐂 a b f.
   HB.instance Definition _ := _iso.
 HB.end.
 
-#[short(type="mclane")]
-HB.structure Definition Mclane (𝐂: PreMonoidalCat) A B :=
-  { f of isMcLane 𝐂 A B f }.
+#[short(type="maclane")]
+HB.structure Definition Maclane (𝐂: PreMonoidalCat) A B :=
+  { f of isMacLane 𝐂 A B f }.
 Arguments src_gtree {_ _ _}.
 Arguments tgt_gtree {_ _ _}.
 Arguments rmcl {_ _ _}.
 
-Definition src_tree {𝐂: PreMonoidalCat} (A B: 𝐂) (f: mclane A B) := gtree_tree (src_gtree f).
-Definition tgt_tree {𝐂: PreMonoidalCat} (A B: 𝐂) (f: mclane A B) := gtree_tree (tgt_gtree f).
+Definition src_tree {𝐂: PreMonoidalCat} (A B: 𝐂) (f: maclane A B) := gtree_tree (src_gtree f).
+Definition tgt_tree {𝐂: PreMonoidalCat} (A B: 𝐂) (f: maclane A B) := gtree_tree (tgt_gtree f).
 
-Definition compatible {𝐂: PreMonoidalCat} {A B: 𝐂} (f g: mclane A B) :=
+Definition compatible {𝐂: PreMonoidalCat} {A B: 𝐂} (f g: maclane A B) :=
   src_tree f = src_tree g /\ tgt_tree f = tgt_tree g.
   
-Lemma McLane_cs {𝐂: MonoidalCat} {A B: 𝐂} (f g: mclane A B):
+Lemma MacLane_cs {𝐂: MonoidalCat} {A B: 𝐂} (f g: maclane A B):
   compatible f g -> f ≡ g.
 Proof.
   move=>[e e']. rewrite 2!rmorE.
   set rf := rmcl f. 
   set rg := rmcl g.
-  unfold gmclane in *. 
-  have: eval_mclane (cast2' rf e e') ≡ eval_mclane rg by exact/McLane.
-  rewrite eval_mclane_cast !eval_gmclaneE 2!hcastI.
-  move=><-. rewrite hcastI. McLane.
+  unfold gmaclane in *. 
+  have: eval_maclane (cast2' rf e e') ≡ eval_maclane rg by exact/MacLane.
+  rewrite eval_maclane_cast !eval_gmaclaneE 2!hcastI.
+  move=><-. rewrite hcastI. MacLane.
 Qed.
-Arguments McLane_cs {_ _ _} _ _ & _. 
+Arguments MacLane_cs {_ _ _} _ _ & _. 
 
 
 (** tweaking coercions to use [eval_gtree] from [gtree] also to classes before [premonoidalcat.sort]
@@ -387,12 +397,12 @@ Implicit Types A B C D: 𝐂.
 Implicit Types a b c d: gtree 𝐂.  
 
 Program Definition _mcl_id a :=
-  @isMcLane.Build 𝐂 a a idmap
+  @isMacLane.Build 𝐂 a a idmap
     a a erefl erefl
     (gmcl_id _) _. 
-Next Obligation. intro a=>/=. by rewrite eval_gmclane_id. Qed.
+Next Obligation. intro a=>/=. by rewrite eval_gmaclane_id. Qed.
 HB.instance Definition _ a := @_mcl_id a.
-Definition mclane_id a: mclane a a := idmap. 
+Definition maclane_id a: maclane a a := idmap. 
 
 Lemma hcast_comp_src A B B' C A' B'' C' (f: A ~> B) (g: B' ~> C) 
   (a: A=A') (b: B=B'') (b': B'=B'') (c: C=C'):
@@ -407,284 +417,284 @@ Proof. by destruct a; destruct b; destruct b'; destruct c. Qed.
 Lemma hcast_gtree_src a' a B (e: gtree_tree a' = gtree_tree a) (e': eval_gtree a = eval_gtree a') (f: a ~> B): hcast' f e' erefl ≡ f ∘ mcl_eq e.
 Proof.
   rewrite /mcl_eq. destruct (esym _), (etrans _ _). 
-  rewrite (UIP_ob _ _ e' erefl)/=. cat.
+  rewrite (UIP_ob e' erefl)/=. cat.
 Qed.
 
 Lemma hcast_gtree_tgt A b b' (e: gtree_tree b = gtree_tree b') (e': eval_gtree b = eval_gtree b') (f: A ~> b): hcast' f erefl e' ≡ mcl_eq e ∘ f.
 Proof.
   rewrite /mcl_eq. destruct (esym _), (etrans _ _). 
-  rewrite (UIP_ob _ _ e' erefl)/=. cat.
+  rewrite (UIP_ob e' erefl)/=. cat.
 Qed.  
 
-Program Definition _mcl_comp A B C (f: mclane A B) (g: mclane B C)
+Program Definition _mcl_comp A B C (f: maclane A B) (g: maclane B C)
   (e: tgt_tree f = src_tree g)
   :=
-  @isMcLane.Build 𝐂 A C (g ∘ f)
+  @isMacLane.Build 𝐂 A C (g ∘ f)
     (src_gtree f) (tgt_gtree g) srcE tgtE
     (gmcl_comp' (rmcl f) e (rmcl g))
     _.
 Next Obligation. 
   intros A B C f g e.
-  rewrite 2!rmorE eval_gmclane_comp'.
+  rewrite 2!rmorE eval_gmaclane_comp'.
   by rewrite hcast_comp_tgt -hcast_gtree_src. 
 Qed.
 HB.instance Definition _ A B C f g e := @_mcl_comp A B C f g e.
-#[refine] Definition mclane_comp A B C (f: mclane A B) (g: mclane B C) (e: tgt_tree f = src_tree g):
-  mclane A C := f \; g.
+#[refine] Definition maclane_comp A B C (f: maclane A B) (g: maclane B C) (e: tgt_tree f = src_tree g):
+  maclane A C := f \; g.
 Proof. done. Defined.
 
-Program Definition _mcl_tensor A B C D (f: mclane A B) (g: mclane C D) :=
-  @isMcLane.Build _ _ _ (f·g)
-    (gt_tens (src_gtree f) (src_gtree g))
-    (gt_tens (tgt_gtree f) (tgt_gtree g))
+Program Definition _mcl_tensor A B C D (f: maclane A B) (g: maclane C D) :=
+  @isMacLane.Build _ _ _ (f·g)
+    (gt_tensor (src_gtree f) (src_gtree g))
+    (gt_tensor (tgt_gtree f) (tgt_gtree g))
     (tensor11_eq srcE srcE)
     (tensor11_eq tgtE tgtE)
     (gmcl_tensor (rmcl f) (rmcl g)) _.
 Next Obligation.
   intros a b c d f g. rewrite 2!rmorE.
-  rewrite hcast_tensor eval_gmclane_tensor. McLane. 
+  rewrite hcast_tensor eval_gmaclane_tensor. MacLane. 
 Qed.
 HB.instance Definition _ A B C D f g := @_mcl_tensor A B C D f g.
-Definition mclane_tensor A B C D (f: mclane A B) (g: mclane C D):
-  mclane _ _ := f · g.
+Definition maclane_tensor A B C D (f: maclane A B) (g: maclane C D):
+  maclane _ _ := f · g.
 
-Program Definition _mcl_inv A B (f: mclane A B) :=
-  @isMcLane.Build _ _ _ (f⁻¹)
+Program Definition _mcl_inv A B (f: maclane A B) :=
+  @isMacLane.Build _ _ _ (f⁻¹)
     (tgt_gtree f) (src_gtree f) tgtE srcE
     (gmcl_inv (rmcl f)) _.
 Next Obligation.
   intros a b f.
-  rewrite eval_gmclane_inv hcast_inv. apply/inv_eqv.
+  rewrite eval_gmaclane_inv hcast_inv. apply/inv_eqv.
   move: (@rmorE _ _ _ f). by rewrite hcast_iso. 
 Qed.
 HB.instance Definition _ A B f := @_mcl_inv A B f.
-Definition mclane_inv A B (f: mclane A B):
-  mclane _ _ := inv f.
+Definition maclane_inv A B (f: maclane A B):
+  maclane _ _ := inv f.
 
 Program Definition _mcl_assoc a b c :=
-  @isMcLane.Build _ ((a ⊗ b) ⊗ c) (a ⊗ b ⊗ c) (assoc a b c)
-    (gt_tens (gt_tens a b) c) (gt_tens a (gt_tens b c)) _ _ 
+  @isMacLane.Build _ ((a ⊗ b) ⊗ c) (a ⊗ b ⊗ c) (assoc a b c)
+    (gt_tensor (gt_tensor a b) c) (gt_tensor a (gt_tensor b c)) _ _ 
     (gmcl_assoc a b c) _.
 Next Obligation. intros=>//=; by rewrite 3!roE. Qed.
 Next Obligation. intros=>//=; by rewrite 3!roE. Qed.
-Next Obligation. intros. rewrite eval_gmclane_assoc hcast_assoc_//; apply: roE. Qed.
+Next Obligation. intros. rewrite eval_gmaclane_assoc hcast_assoc_//; apply: roE. Qed.
 HB.instance Definition _ a b c := @_mcl_assoc a b c.
-HB.instance Definition _ a b c := Mclane.on (assoc' a b c).
-Definition mclane_assoc a b c: mclane _ _ := assoc a b c.
-Definition mclane_assoc' a b c: mclane _ _ := assoc' a b c.
+HB.instance Definition _ a b c := Maclane.on (assoc' a b c).
+Definition maclane_assoc a b c: maclane _ _ := assoc a b c.
+Definition maclane_assoc' a b c: maclane _ _ := assoc' a b c.
 
 Program Definition _mcl_unitl a :=
-  @isMcLane.Build _ _ _ (unitl a)
-    (gt_tens gt_unit a) a _ _ 
+  @isMacLane.Build _ _ _ (unitl a)
+    (gt_tensor gt_unit a) a _ _ 
     (gmcl_unitl _) _.
 Next Obligation. intros=>//=; by rewrite roE. Qed.
 Next Obligation. intros=>//=; by rewrite roE. Qed.
-Next Obligation. intros. by rewrite eval_gmclane_unitl hcast_unitl_. Qed.
+Next Obligation. intros. by rewrite eval_gmaclane_unitl hcast_unitl_. Qed.
 HB.instance Definition _ a := @_mcl_unitl a.
-HB.instance Definition _ a := Mclane.on (unitl' a).
-Definition mclane_unitl a: mclane _ _ := unitl a.
-Definition mclane_unitl' a: mclane _ _ := unitl' a.
+HB.instance Definition _ a := Maclane.on (unitl' a).
+Definition maclane_unitl a: maclane _ _ := unitl a.
+Definition maclane_unitl' a: maclane _ _ := unitl' a.
 
 Program Definition _mcl_unitr a :=
-  @isMcLane.Build _ _ _ (unitr a)
-    (gt_tens a gt_unit) a _ _
+  @isMacLane.Build _ _ _ (unitr a)
+    (gt_tensor a gt_unit) a _ _
     (gmcl_unitr _) _.
 Next Obligation. intros=>//=; by rewrite roE. Qed.
 Next Obligation. intros=>//=; by rewrite roE. Qed.
-Next Obligation. intros. by rewrite eval_gmclane_unitr hcast_unitr_. Qed.
+Next Obligation. intros. by rewrite eval_gmaclane_unitr hcast_unitr_. Qed.
 HB.instance Definition _ a := @_mcl_unitr a.
-HB.instance Definition _ a := Mclane.on (unitr' a).
-Definition mclane_unitr a: mclane _ _ := unitr a.
-Definition mclane_unitr' a: mclane _ _ := unitr' a.
+HB.instance Definition _ a := Maclane.on (unitr' a).
+Definition maclane_unitr a: maclane _ _ := unitr a.
+Definition maclane_unitr' a: maclane _ _ := unitr' a.
 
-Program Definition _mcl_bcomp A B B' C (f: mclane A B) (m: mclane B B') (g: mclane B' C) 
+Program Definition _mcl_bcomp A B B' C (f: maclane A B) (m: maclane B B') (g: maclane B' C) 
   (i: tgt_tree f = src_tree m)
   (j: tgt_tree m = src_tree g)
   :=
-  @isMcLane.Build 𝐂 A C (bcomp f g m)
+  @isMacLane.Build 𝐂 A C (bcomp f g m)
     (src_gtree f) (tgt_gtree g) srcE tgtE
     (gmcl_comp' (rmcl f) i (gmcl_comp' (rmcl m) j (rmcl g))) _.
 Next Obligation.
   intros a b b' c f m g i j. rewrite /bcomp-lock/=.
-  rewrite 3!rmorE 2!eval_gmclane_comp'.
+  rewrite 3!rmorE 2!eval_gmaclane_comp'.
   by rewrite 2!hcast_comp_tgt -2!hcast_gtree_src.
 Qed.
 HB.instance Definition _ A B B' C f g m i j := @_mcl_bcomp A B B' C f g m i j.
-#[refine] Definition mclane_bcomp A B B' C (f: mclane A B) (m: mclane B B') (g: mclane B' C)
+#[refine] Definition maclane_bcomp A B B' C (f: maclane A B) (m: maclane B B') (g: maclane B' C)
   (i: tgt_tree f = src_tree m)
   (j: tgt_tree m = src_tree g):
-  mclane A C := bcomp f g m.
+  maclane A C := bcomp f g m.
 Proof. all: done. Defined.
 
-Program Definition _mcl_cast A B B' C (f: mclane A B) (m: mclane B B') (g: mclane B' C) 
+Program Definition _mcl_cast A B B' C (f: maclane A B) (m: maclane B B') (g: maclane B' C) 
   (i: tgt_tree f = src_tree m)
   (j: tgt_tree m = src_tree g)
   :=
-  @isMcLane.Build 𝐂 A C (cast' f g m)
+  @isMacLane.Build 𝐂 A C (cast' f g m)
     (src_gtree f) (tgt_gtree g) srcE tgtE
     (gmcl_comp' (rmcl f) i (gmcl_comp' (rmcl m) j (rmcl g))) _.
 Next Obligation.
   intros a b b' c f m g i j. rewrite /cast-lock/=.
-  rewrite 3!rmorE 2!eval_gmclane_comp'.
+  rewrite 3!rmorE 2!eval_gmaclane_comp'.
   by rewrite 2!hcast_comp_tgt -2!hcast_gtree_src.
 Qed.
 HB.instance Definition _ A B B' C f g m i j := @_mcl_cast A B B' C f g m i j.
-#[refine] Definition mclane_cast A B B' C (f: mclane A B) (m: mclane B B') (g: mclane B' C)
+#[refine] Definition maclane_cast A B B' C (f: maclane A B) (m: maclane B B') (g: maclane B' C)
   (i: tgt_tree f = src_tree m)
   (j: tgt_tree m = src_tree g):
-  mclane A C := cast' f g m.
+  maclane A C := cast' f g m.
 Proof. all: done. Defined.
 
-Program Definition _mcl_eval_gmclane (s t: gtree 𝐂) (h: gmclane s t)
-  := @isMcLane.Build _ (eval_gtree s) (eval_gtree t) (eval_gmclane h)
+Program Definition _mcl_eval_gmaclane (s t: gtree 𝐂) (h: gmaclane s t)
+  := @isMacLane.Build _ (eval_gtree s) (eval_gtree t) (eval_gmaclane h)
        s t erefl erefl
        h _.
 Next Obligation. intros. by rewrite hcastK. Qed.
-HB.instance Definition _ s t h := @_mcl_eval_gmclane s t h.
-Definition mclane_eval_gmclane s t (h: gmclane s t): mclane _ _ := eval_gmclane h.
+HB.instance Definition _ s t h := @_mcl_eval_gmaclane s t h.
+Definition maclane_eval_gmaclane s t (h: gmaclane s t): maclane _ _ := eval_gmaclane h.
 
-Program Definition _mcl_eval_mclane (s t: tree 𝐂) (h: monoidal_mclane.mclane s t)
-  := @isMcLane.Build _ (eval_tree s) (eval_tree t) (eval_mclane h)
+Program Definition _mcl_eval_maclane (s t: tree 𝐂) (h: monoidal_maclane.maclane s t)
+  := @isMacLane.Build _ (eval_tree s) (eval_tree t) (eval_maclane h)
        (tree_gtree s) (tree_gtree t) (esym (eval_tree_gtree s)) (esym (eval_tree_gtree t))
-       (gmcl_mclane h) _.
-Next Obligation. intros. by rewrite eval_gmclane_mclane hcastI hcastK. Qed.
-HB.instance Definition _ s t h := @_mcl_eval_mclane s t h.
-Definition mclane_eval_mclane s t (h: monoidal_mclane.mclane s t): mclane _ _ := eval_mclane h.
+       (gmcl_maclane h) _.
+Next Obligation. intros. by rewrite eval_gmaclane_maclane hcastI hcastK. Qed.
+HB.instance Definition _ s t h := @_mcl_eval_maclane s t h.
+Definition maclane_eval_maclane s t (h: monoidal_maclane.maclane s t): maclane _ _ := eval_maclane h.
 
 End s.
-Arguments mclane_comp {_ _ _ _} _ _&.
-Arguments mclane_bcomp {_ _ _ _ _} _ _ _&.
-Arguments mclane_cast {_ _ _ _ _} _ _ _&.
+Arguments maclane_comp {_ _ _ _} _ _&.
+Arguments maclane_bcomp {_ _ _ _ _} _ _ _&.
+Arguments maclane_cast {_ _ _ _ _} _ _ _&.
 
 Ltac reify_gmcl f :=
   lazymatch f with
   | idmap ?A =>
       let a := reify_ob A in
-      constr:(mclane_id a)
+      constr:(maclane_id a)
   | ?f \; ?g =>
       let u := reify_gmcl f in
       let v := reify_gmcl g in
-      uconstr:(mclane_comp u v _)
+      uconstr:(maclane_comp u v _)
   | inv ?f =>
       let f := (eval simpl in (iso.sort f)) in
       let u := reify_gmcl f in
-      uconstr:(mclane_inv u)
+      uconstr:(maclane_inv u)
   | ?f · ?g =>
       let u := reify_gmcl f in
       let v := reify_gmcl g in
-      uconstr:(mclane_tensor u v)
+      uconstr:(maclane_tensor u v)
   | assoc ?A ?B ?C =>
       let a := reify_ob A in
       let b := reify_ob B in
       let c := reify_ob C in
-      constr:(mclane_assoc a b c)
+      constr:(maclane_assoc a b c)
   | assoc' ?A ?B ?C =>
       let a := reify_ob A in
       let b := reify_ob B in
       let c := reify_ob C in
-      constr:(mclane_assoc' a b c)
+      constr:(maclane_assoc' a b c)
   | unitl ?A =>
       let a := reify_ob A in
-      constr:(mclane_unitl a)
+      constr:(maclane_unitl a)
   | unitl' ?A =>
       let a := reify_ob A in
-      constr:(mclane_unitl' a)
+      constr:(maclane_unitl' a)
   | unitr ?A =>
       let a := reify_ob A in
-      constr:(mclane_unitr a)
+      constr:(maclane_unitr a)
   | unitr' ?A =>
       let a := reify_ob A in
-      constr:(mclane_unitr' a)
+      constr:(maclane_unitr' a)
   | bcomp ?f ?g ?m =>
       let u := reify_gmcl f in
       let v := reify_gmcl g in
       let w := reify_gmcl m in
-      uconstr:(mclane_bcomp u w v _ _)
+      uconstr:(maclane_bcomp u w v _ _)
   | cast' ?f ?g ?m =>
       let u := reify_gmcl f in
       let v := reify_gmcl g in
       let w := reify_gmcl m in
-      uconstr:(mclane_cast u w v _ _)
+      uconstr:(maclane_cast u w v _ _)
   | blocked_id ?A =>
       let a := reify_ob A in
-      constr:(mclane_id a)
+      constr:(maclane_id a)
   | blocked_comp ?f ?g =>
       let u := reify_gmcl f in
       let v := reify_gmcl g in
-      uconstr:(mclane_comp u v _)
+      uconstr:(maclane_comp u v _)
   | blocked_inv ?f =>
       let f := (eval simpl in (iso.sort f)) in
       let u := reify_gmcl f in
-      uconstr:(mclane_inv u)
+      uconstr:(maclane_inv u)
   | blocked_tens ?f ?g =>
       let u := reify_gmcl f in
       let v := reify_gmcl g in
-      uconstr:(mclane_tensor u v)
+      uconstr:(maclane_tensor u v)
   | @blocked_assoc _ ?A ?B ?C =>
       let a := reify_ob A in
       let b := reify_ob B in
       let c := reify_ob C in
-      constr:(mclane_assoc a b c)
+      constr:(maclane_assoc a b c)
   | @blocked_assoc' _ ?A ?B ?C =>
       let a := reify_ob A in
       let b := reify_ob B in
       let c := reify_ob C in
-      constr:(mclane_assoc' a b c)
+      constr:(maclane_assoc' a b c)
   | @blocked_unitl _ ?A =>
       let a := reify_ob A in
-      constr:(mclane_unitl a)
+      constr:(maclane_unitl a)
   | @blocked_unitl' _ ?A =>
       let a := reify_ob A in
-      constr:(mclane_unitl' a)
+      constr:(maclane_unitl' a)
   | @blocked_unitr _ ?A =>
       let a := reify_ob A in
-      constr:(mclane_unitr a)
+      constr:(maclane_unitr a)
   | @blocked_unitr' _ ?A =>
       let a := reify_ob A in
-      constr:(mclane_unitr' a)
+      constr:(maclane_unitr' a)
   | iso.sort ?f => reify_gmcl f
   | reverse_coercion ?f _ => reify_gmcl f
   | mcl ?f => reify_gmcl f
-  | iso_gmclane ?m => constr:(mclane_eval_gmclane m)
-  | eval_gmclane ?m => constr:(mclane_eval_gmclane m)
-  | eval_mclane ?m => constr:(mclane_eval_mclane m)
-  | Mclane.sort ?m => constr:(m)
-  | _ => fail "could not reify" f "as a McLane morphism" 
+  | iso_gmaclane ?m => constr:(maclane_eval_gmaclane m)
+  | eval_gmaclane ?m => constr:(maclane_eval_gmaclane m)
+  | eval_maclane ?m => constr:(maclane_eval_maclane m)
+  | Maclane.sort ?m => constr:(m)
+  | _ => fail "could not reify" f "as a MacLane morphism" 
   end.
 
-Ltac gMcLane_gen tac :=
+Ltac gMacLane_gen tac :=
   unfold auto_eqv; 
-  let rec gMcLane := 
+  let rec gMacLane := 
     try reflexivity;
     rewrite /=;
     match goal with
-    | |- comp _ _ ≡ comp _ _ => apply: comp_eqv; gMcLane
-    | |- bcomp _ _ _ ≡ bcomp _ _ _ => apply: bcomp_eqv; gMcLane
-    | |- tensor22 _ _ ≡ tensor22 _ _ => apply: tensor_eqv; gMcLane
-    | |- hcast _ ≡ hcast _ => apply: hcast_eqv'; gMcLane
-    | |- cast _ ≡ cast _ => apply: cast_eqv; gMcLane
+    | |- comp _ _ ≡ comp _ _ => apply: comp_eqv; gMacLane
+    | |- bcomp _ _ _ ≡ bcomp _ _ _ => apply: bcomp_eqv; gMacLane
+    | |- tensor22 _ _ ≡ tensor22 _ _ => apply: tensor_eqv; gMacLane
+    | |- hcast _ ≡ hcast _ => apply: hcast_eqv'; gMacLane
+    | |- cast _ ≡ cast _ => apply: cast_eqv; gMacLane
     | |- ?f ≡ ?g =>
         let u := reify_gmcl f in
         let v := reify_gmcl g in
         tac u v
     end
-  in gMcLane.
-Ltac gMcLane_try_ u v :=
-  unshelve refine (McLane_cs u v _)=>//=;
+  in gMacLane.
+Ltac gMacLane_try_ u v :=
+  unshelve refine (MacLane_cs u v _)=>//=;
     (try split); rewrite /=?tensor_arity_app//=.
-Ltac gMcLane_solve u v := by gMcLane_try_ u v.
-Ltac gMcLane_pose_ u v := epose (McLane_cs u v _)=>//=.
-Ltac gMcLane := gMcLane_gen gMcLane_solve.
-Ltac gMcLane_try := gMcLane_gen gMcLane_try_.
-Ltac gMcLane_pose := gMcLane_gen gMcLane_pose_.
+Ltac gMacLane_solve u v := by gMacLane_try_ u v.
+Ltac gMacLane_pose_ u v := epose (MacLane_cs u v _)=>//=.
+Ltac gMacLane := gMacLane_gen gMacLane_solve.
+Ltac gMacLane_try := gMacLane_gen gMacLane_try_.
+Ltac gMacLane_pose := gMacLane_gen gMacLane_pose_.
 
-#[export] Hint Extern 0 (auto_eqv _ _) => gMcLane: typeclass_instances.
+#[export] Hint Extern 0 (auto_eqv _ _) => gMacLane: typeclass_instances.
 
-Arguments eval_mclane: simpl never.
-Arguments iso_gmclane: simpl never.
-Arguments eval_gmclane: simpl never.
+Arguments eval_maclane: simpl never.
+Arguments iso_gmaclane: simpl never.
+Arguments eval_gmaclane: simpl never.
 
-Section tests_gMcLane.
+Section tests_gMacLane.
   
 Context {𝐂: MonoidalCat}.
 Variables A B C D: 𝐂.
@@ -692,88 +702,88 @@ Variables a b c d: tree 𝐂.
 Variables h k l Γ Δ: arity 𝐂.
 
 Goal A ≡ A.
-Proof. gMcLane. Qed.
+Proof. gMacLane. Qed.
 Goal A·B ≡ A·B.
-Proof. gMcLane. Qed.
+Proof. gMacLane. Qed.
 Goal unitl A \; unitl' A ≡ idmap.
-Proof. gMcLane. Qed.
+Proof. gMacLane. Qed.
 Goal assoc A B C ≡ assoc A B C.
-Proof. gMcLane. Qed.
+Proof. gMacLane. Qed.
 Goal A · assoc B C D ∘ assoc A (B⊗C) D ∘ assoc A B C · D
      ≡ assoc A B (C⊗D) ∘ assoc (A⊗B) C D.
-Proof. gMcLane. Qed.
+Proof. gMacLane. Qed.
 
 Goal A · unitl B ∘ assoc A unit B ≡ unitr A · B.
-Proof. gMcLane. Qed.
+Proof. gMacLane. Qed.
 
 Goal A · unitl (B⊗C) ∘ assoc A unit (B⊗C) ≡ unitr A · (B⊗C).
-Proof. gMcLane. Qed.
+Proof. gMacLane. Qed.
 
 Goal A · unitl (B⊗C) ∘ assoc A unit (B⊗C) ≡ mcl.
-Proof. gMcLane. Qed.
+Proof. gMacLane. Qed.
 
 Goal idmap h ≡ mcl.
-Proof. gMcLane. Qed.
+Proof. gMacLane. Qed.
 
 Goal idmap h ≡ mcl ∘ idmap.
-Proof. gMcLane. Qed.
+Proof. gMacLane. Qed.
 
 Goal A · unitl h ∘ assoc A unit h ≡ unitr A · eval_arity h.
-Proof. gMcLane. Qed.
+Proof. gMacLane. Qed.
 
 Goal acast (A · unitl h) ≡ unitr A · eval_arity h.
-Proof. gMcLane. Qed.
+Proof. gMacLane. Qed.
 
 Goal assoc A B C ∘∘ assoc A B C ≡ mcl.
-Proof. gMcLane. Qed.
+Proof. gMacLane. Qed.
 
 Goal unitl unit ≡[𝐂 _ _] unitr unit. 
-Proof. gMcLane. Qed.
+Proof. gMacLane. Qed.
 
 Goal unitl A ≡ inv (unitl' A). 
-Proof. gMcLane. Qed.
+Proof. gMacLane. Qed.
 
 Goal inv (unitl (A⊗B)) ≡ mcl. 
-Proof. gMcLane. Qed.
+Proof. gMacLane. Qed.
 
-Goal forall (s t: gtree 𝐂) (i: mclane s t), i ∘ inv i ≡ idmap. 
-Proof. intros. gMcLane_try. unfold compatible. cbn. Abort.
+Goal forall (s t: gtree 𝐂) (i: maclane s t), i ∘ inv i ≡ idmap. 
+Proof. intros. gMacLane_try. unfold compatible. cbn. Abort.
 
-(* Notation test_mclane f := (f ≡ idmap ∘ f) (only parsing). *)
-Notation test_mclane f := (f ∘ inv f ≡ idmap) (only parsing).
+(* Notation test_maclane f := (f ≡ idmap ∘ f) (only parsing). *)
+Notation test_maclane f := (f ∘ inv f ≡ idmap) (only parsing).
 
-Goal test_mclane (mcl: h⊗unit ≃ h).
-Proof. gMcLane. Qed.
+Goal test_maclane (mcl: h⊗unit ≃ h).
+Proof. gMacLane. Qed.
 
-Goal test_mclane (mcl: h⊗unit ~> h).
-Proof. gMcLane. Qed.
+Goal test_maclane (mcl: h⊗unit ~> h).
+Proof. gMacLane. Qed.
   
-Goal test_mclane (mcl: (h++k)⊗B ~> h⊗k⊗B⊗unit).
-Proof. gMcLane. Qed.
+Goal test_maclane (mcl: (h++k)⊗B ~> h⊗k⊗B⊗unit).
+Proof. gMacLane. Qed.
 
-Goal test_mclane (mcl: h++A⊗unit⊗B::k ~> h⊗A⊗B⊗k).
-Proof. gMcLane. Qed.
+Goal test_maclane (mcl: h++A⊗unit⊗B::k ~> h⊗A⊗B⊗k).
+Proof. gMacLane. Qed.
 
-Goal test_mclane (mcl: unit ⊗ Nf b ⊗ C ~> b ⊗ C).
-Proof. gMcLane. Qed.
+Goal test_maclane (mcl: unit ⊗ Nf b ⊗ C ~> b ⊗ C).
+Proof. gMacLane. Qed.
 
-Goal test_mclane (mcl: unit ⊗ Nf (t_tens b c) ⊗ C ~> b ⊗ c ⊗ C).
-Proof. gMcLane. Qed.
+Goal test_maclane (mcl: unit ⊗ Nf (t_tensor b c) ⊗ C ~> b ⊗ c ⊗ C).
+Proof. gMacLane. Qed.
 
-Goal test_mclane (mcl: unit ⊗ Nf (t_tens b c) ⊗ C ~> b ⊗ Nf c ⊗ C).
-Proof. gMcLane. Qed.
+Goal test_maclane (mcl: unit ⊗ Nf (t_tensor b c) ⊗ C ~> b ⊗ Nf c ⊗ C).
+Proof. gMacLane. Qed.
 
-Goal test_mclane (mcl: unit ⊗ (h++k) ⊗ B ⊗ C ~> h ⊗ unit ⊗ k ⊗ B ⊗ unit ⊗ C).
-Proof. gMcLane. Qed.
+Goal test_maclane (mcl: unit ⊗ (h++k) ⊗ B ⊗ C ~> h ⊗ unit ⊗ k ⊗ B ⊗ unit ⊗ C).
+Proof. gMacLane. Qed.
 
-Goal test_mclane (mcl: A ⊗ (h++B::k) ⊗ C ~> A⊗ h ⊗ B ⊗ k ⊗ unit ⊗ C).
-Proof. gMcLane. Qed.
+Goal test_maclane (mcl: A ⊗ (h++B::k) ⊗ C ~> A⊗ h ⊗ B ⊗ k ⊗ unit ⊗ C).
+Proof. gMacLane. Qed.
 
-Goal test_mclane (mcl: A ⊗ (h++(B⊗C)::k) ⊗ C ~> A⊗ h ⊗ B ⊗ C ⊗ k ⊗ unit ⊗ C).
-Proof. gMcLane. Qed.
+Goal test_maclane (mcl: A ⊗ (h++(B⊗C)::k) ⊗ C ~> A⊗ h ⊗ B ⊗ C ⊗ k ⊗ unit ⊗ C).
+Proof. gMacLane. Qed.
 
-Goal test_mclane (mcl: A ⊗ (h++(B⊗l)::k) ⊗ C ~> A⊗ h ⊗ B ⊗ l ⊗ k ⊗ unit ⊗ C).
-Proof. gMcLane. Qed.
+Goal test_maclane (mcl: A ⊗ (h++(B⊗l)::k) ⊗ C ~> A⊗ h ⊗ B ⊗ l ⊗ k ⊗ unit ⊗ C).
+Proof. gMacLane. Qed.
 
-End tests_gMcLane.
+End tests_gMacLane.
 
