theories/adjunction.v
@@ -5,10 +5,12 @@ Require Export functor.
 Local Open Scope cat_scope.
 
 (** ** indexed by the left adjoint *)
-#[primitive] HB.mixin Record isLeftAdjoint {𝐂 𝐃: Cat} (F: 𝐂 ~> 𝐃) (* F of @functor 𝐂 𝐃 F *) :=
-  { #[canonical=no] radj: 𝐃 ~> 𝐂; 
-    #[canonical=no] unit: idmap 𝐂 ~> radj ∘ F;
-    #[canonical=no] counit: F ∘ radj ~> idmap 𝐃;
+
+(*TMP-UNIV: revert to nice notations *)
+#[primitive] HB.mixin Record isLeftAdjoint {𝐂 𝐃: Cat} (F: 𝐂 ≈> 𝐃) (* F of @functor 𝐂 𝐃 F *) :=
+  { #[canonical=no] radj: 𝐃 ≈> 𝐂; 
+    #[canonical=no] unit: functor_id ~> functor_comp F radj;
+    #[canonical=no] counit: functor_comp radj F ~> functor_id;
     #[canonical=no] counit_unit: idmap ⊚ counit ∘ unit ⊚ idmap ≡ ntx_id _;
     #[canonical=no] unit_counit: idmap ⊚ unit ∘ counit ⊚ idmap ≡ ntx_id _;
   }.
