theories/cat_cat.v
@@ -1,0 +1,103 @@
+(** * the Cartesian category of categories *)
+
+(* we isolate this part of the library for now:
+   its needs universe polymorphism, which is not supported by HB, yet
+   as a workaround, we temporarily deactivate universe-checking
+ *)
+Require Export span functor product.
+
+Local Open Scope cat_scope.
+
+Unset Universe Checking.
+
+HB.instance Definition _ := IsQuiver.Build Cat Functor.
+HB.instance Definition _ := IsPreCat.Build Cat (@functor_id) (@functor_comp).
+
+Program Definition _cat_cat := IsCat.Build Cat _ _ _ _.
+Next Obligation. split. exact: same_functor. Qed.
+Next Obligation. split. exact: same_functor. Qed.
+Next Obligation. split. exact: same_functor. Qed.
+Next Obligation. intros. exact: functor_comp_eqv. Qed.
+HB.instance Definition _ := _cat_cat.
+
+Definition cat_top: Terminal Cat.
+  exists (Cat1: Cat)=>X.
+  unshelve eexists=>//.
+  exact (functor_cst (tt: Cat1)).
+  move=>F _/=. split.
+  repeat unshelve eexists. 
+Defined.
+
+Definition cat_prod (C D: Cat): Product C D.
+  unshelve eexists.
+  exists (C * D: Cat)%type.
+  exact: (Datatypes.fst: Functor _ _). 
+  exact: (Datatypes.snd: Functor _ _).
+  unshelve eexists=>//. 
+  exists ((types_pair' (spanl (s:=X)) (spanr (s:=X))): Functor _ _).
+  split; split; exact: same_functor.
+  destruct X as [X L R]=>/=[[F [[HL] [HR]]]] _. cbn. split.
+  apply: iso_trans. apply: types_pair'_iso; apply: iso_sym; eassumption.
+  clear. unshelve apply: mk_iso.
+  { unshelve eexists.
+    - split; exact: idmap; split; split; split=>/=; cat.
+    - repeat split=>/=; cat. }
+  { unshelve eexists.
+    - split; exact: idmap; split; split; split=>/=; cat.
+    - repeat split=>/=; cat. }
+  split=>/=; cat. 
+  split=>/=; cat. 
+Defined.
+HB.instance Definition _ := IsCartesian.Build Cat cat_top cat_prod.
+
+Unset Universe Checking.
+
+Definition times {X X' Y Y': Cat}
+  (f: X ~> X') (g: Y ~> Y'): X×Y ~> X'×Y' :=
+  app22 (@PROD Cat: Functor _ _) f g.
+Instance times_eqv {X X' Y Y'}: Proper (eqv ==> eqv ==> eqv) (@times X X' Y Y').
+Proof. apply (app22_eqv (F:=@PROD Cat: Functor _ _)). Qed.
+
+(** a nicer definition for premonoidal categories *)
+
+#[primitive] HB.factory Record IsPreMonoidal' 𝐂 of cat 𝐂 := {
+    #[canonical=no] unit: 𝐂;
+    #[canonical=no] tensor: (𝐂*𝐂)%type ≈> 𝐂;
+    
+    (* w.r.t nlab: https://ncatlab.org/nlab/show/monoidal+category *)
+    (*    assoc = α, unitl = λ, unitr = ρ *)
+    #[canonical=no] assoc_:
+    tensor ∘ times tensor idmap
+      ≈
+    tensor ∘ times idmap tensor ∘ (prod_assoc _ _ _)¹;
+    #[canonical=no] unitl_:
+    tensor ∘ (times (functor_cst unit) idmap)
+      ≈
+    (@prod_unitl Cat _)¹;
+    #[canonical=no] unitr_: 
+    tensor ∘ (times idmap (functor_cst unit))
+      ≈
+    (@prod_unitr Cat _)¹;
+  }.
+
+(*
+Lemma ntx_assoc [A B A' B' A'' B''] (f: A ~> B) (g: A' ~> B') (h: A'' ~> B''):
+  assoc _ _ _ ∘ (f · g) · h ≡ f · (g · h) ∘ assoc _ _ _.
+Proof. exact: (@natural _ _ _ _ (assoc_¹) (_,_,_) (_,_,_) (f,g,h)). Qed.
+
+Lemma ntx_assoc' [A B A' B' A'' B''] (f: A ~> B) (g: A' ~> B') (h: A'' ~> B''):
+  assoc' _ _ _ ∘ f · (g · h) ≡ (f · g) · h ∘ assoc' _ _ _.
+Proof. exact: (@natural _ _ _ _ (assoc_⁻¹) (_,_,_) (_,_,_) (f,g,h)). Qed.
+
+Lemma ntx_unitl [A B] (f: A ~> B): unitl _ ∘ unit · f ≡ f ∘ unitl _.
+Proof. exact: (@natural _ _ _ _ (unitl_¹) (tt,A) (tt,B) (idmap,f)). Qed.
+
+Lemma ntx_unitl' [A B] (f: A ~> B): unitl' _ ∘ f ≡ unit · f ∘ unitl' _.
+Proof. exact: (@natural _ _ _ _ (unitl_⁻¹) (tt,A) (tt,B) (idmap,f)). Qed.
+
+Lemma ntx_unitr [A B] (f: A ~> B): unitr _ ∘ f · unit ≡ f ∘ unitr _.
+Proof. exact: (@natural _ _ _ _ (unitr_¹) (A,tt) (B,tt) (f,idmap)). Qed.
+
+Lemma ntx_unitr' [A B] (f: A ~> B): unitr' _ ∘ f ≡ f · unit ∘ unitr' _.
+Proof. exact: (@natural _ _ _ _ (unitr_⁻¹) (A,tt) (B,tt) (f,idmap)). Qed.
+*)
