theories/monoidal_examples.v
@@ -5,6 +5,20 @@ Import NiceNotations.
 
 Local Open Scope cat_scope.
 
+Section warmup.
+
+Context {𝐂: MonoidalCat} (A B C: 𝐂).
+
+Goal forall f: A ⊗ A ~> B, forall g: B ~> C, forall h: B ~> C ⊗ C, (f;g) · h ≡ f·h ; g·C·C.
+Proof. intros. mcat. Qed.
+
+Goal forall f: A ⊗ A ~> B, forall g: B ~> C, forall h: B ~> C ⊗ C, (f;g) · h ≡' f·h ;; (g·C)·C.
+Proof. intros. mcat. Qed.
+
+End warmup.
+
+
+(** ** composing two monoids *)
 Section two.
 
 Context {𝐂: MonoidalCat} (M N: 𝐂).
@@ -12,36 +26,76 @@ Context {𝐂: MonoidalCat} (M N: 𝐂).
 Check mcl: (M⊗N)⊗(M⊗N) ~> M⊗(N⊗M)⊗N.
 
 Variable m: M⊗M ~> M.
+Variable e: unit ~> M.
 Hypothesis mA: m·M ; m ≡' M·m ; m.
+Hypothesis em: e·M ; m ≡' M.
+Hypothesis me: M·e ; m ≡' M.
 
 Variable n: N⊗N ~> N.
+Variable f: unit ~> N.
 Hypothesis nA: n·N ; n ≡' N·n ; n.
+Hypothesis fn: f·N ; n ≡' N.
+Hypothesis nf: N·f ; n ≡' N.
 
 Variable x: N⊗M ~> M⊗N.
 Hypothesis nx: n·M ; x ≡' N·x ;; x·N ;; M·n.
+Hypothesis ex: N·e ; x ≡' e·N.
 Hypothesis mx: N·m ; x ≡' x·M ;; M·x ;; m·N.
+Hypothesis fx: f·M ; x ≡' M·f.
 
 Let mn := M·x·N ;; m·n .
+Let ef := e·f .
 
 Lemma mnA: mn·M·N ;; mn ≡' M·N·mn ;; mn.
 Proof.
   unfold mn.
 
-  transitivity (M·x·N·M·N ;; M·M·[n·M ; x]·N ;; (m·M ; m)·n). mcat.
+  transitivity (M·x·N·M·N ;; M·M·[n·M ; x]·N ;; [m·M ; m]·n). mcat.
   rewrite nx.
-
-  transitivity (M·x·x·N ;; M·M·x·N·N ;; [m·M ; m]·[n·N ; n]). mcat. 
-  rewrite nA.
   rewrite mA.
 
-  transitivity (M·N·M·x·N ;; M·[x·M ;; M·x ;; m·N]·n ;; m·n). mcat.
-  rewrite -mx. 
+  transitivity (M·N·M·x·N ;; M·[N·m ; x]·N·N ;; m·[N·n ; n]). 2: mcat.
+  rewrite mx.
+  rewrite -nA.
 
-  mcat. 
+  mcat.
+Qed.
+
+Lemma efmn: ef·M·N ;; mn ≡' M·N.
+Proof.
+  unfold ef, mn.
+  
+  transitivity ([f·M ; x]·N ;; [e·M ; m]·n). mcat.
+  rewrite fx.
+  rewrite em.
+  
+  transitivity (M·[f·N ; n]). mcat.
+  rewrite fn.
+  
+  mcat.
+Qed.
+
+Lemma mnef: M·N·ef ;; mn ≡' M·N.
+Proof.
+  unfold ef, mn.
+
+  transitivity (M·[N·e ; x] ;; m·[N·f ; n]). mcat.
+  rewrite ex.
+  rewrite nf.
+
+  transitivity ([M·e ; m]·N). mcat.
+  rewrite me.
+  
+  mcat.
 Qed.
 
 End two.
+Print Assumptions mnA.
 
+
+
+
+(** ** composing three monoids (only multiplication here) *)
 Section three.
 
 Context {𝐂: MonoidalCat} (M N O: 𝐂).
@@ -67,6 +121,7 @@ Variable z: O⊗M ~> M⊗O.
 Hypothesis oz: o·M ; z ≡' O·z ;; z·O ;; M·o.
 Hypothesis mz: O·m ; z ≡' z·M ;; M·z ;; m·O.
 
+(* note that we need this additional coherence diagram linking the three distributive laws *)
 Hypothesis xyz: y·M ;; N·z ;; x·O ≡' O·x ;; z·N ;; M·y.
 
 Let mno := M·N·z·N·O ;; M·x·y·O ;; m·n·o.
